Ticketlock proving

src/example/TicketLockRA.v
@@ -4,48 +4,88 @@ From Fairness Require Export AuthExclAnysRA.
 From stdpp Require Import gmap.
 
 
-Section TKLOCK.
+Section Ticket.
 
-  Definition _TicketLockRA : URA.t := URA.prod (Auth.t (URA.prod (Excl.t nat) (GsetK.t (K:=nat)))) AuthExclAnysRA.
-  Definition TicketLockRA : URA.t := (nat ==> _TicketLockRA)%ra.
+  Definition _TicketRA : URA.t := Auth.t (URA.prod (Excl.t nat) (GsetK.t (K:=nat))).
+  Definition TicketRA : URA.t := (nat ==> _TicketRA)%ra.
 
   Context `{Σ : GRA.t}.
-  Context {HasTicketLockRA : @GRA.inG TicketLockRA Σ}.
+  Context {HasTicketRA : @GRA.inG TicketRA Σ}.
 
-  Definition TicketLockRA_Auth_base : _TicketLockRA :=
-    (((@Auth.black (URA.prod _ _) (Some 0 : Excl.t nat, Some ∅ : GsetK.t))
-        ⋅ (@Auth.white (URA.prod _ _) (Some 0 : Excl.t nat, Some ∅ : GsetK.t))),
-      ((fun k => (Auth.black (Some (tt ↑) : Excl.t Any.t) ⋅ Auth.white (Some (tt ↑) : Excl.t Any.t))) : AuthExclAnysRA)
-    ).
+  Definition TicketRA_Auth_base : _TicketRA :=
+    (@Auth.black (URA.prod _ _) (Some 0 : Excl.t nat, Some ∅ : GsetK.t))
+    ⋅ (@Auth.white (URA.prod _ _) (Some 0 : Excl.t nat, Some ∅ : GsetK.t)).
 
-  Definition TicketLockRA_Auth : iProp :=
+  Definition TicketRA_Auth : iProp :=
     (∃ (U : nat), OwnM ((fun k => if (lt_dec k U)
                              then ε
-                             else TicketLockRA_Auth_base) : TicketLockRA)).
+                             else TicketRA_Auth_base) : TicketRA)).
 
+  Definition Ticket_black_ra (r : nat) (o : nat) (D : gset nat) : TicketRA :=
+    maps_to_res r (Auth.black (((Some o) : Excl.t nat, Some D : GsetK.t) : URA.prod _ _)).
+  Definition Ticket_black r o D := OwnM (Ticket_black_ra r o D).
 
-  Definition tklockB_ra (r : nat) (o : nat) (D : gset nat) : TicketLockRA :=
-    (maps_to_res r (((Auth.black (((Some o) : Excl.t nat, Some D : GsetK.t) : URA.prod _ _)),
-                      AuExAny_ra (fun k => gset_elem_of_dec k D)) : URA.prod _ _)).
-  Definition tklockB r o D := OwnM (tklockB_ra r o D).
+  Definition Ticket_locked_ra (r : nat) (o : nat) : TicketRA :=
+    maps_to_res r (Auth.white (((Some o) : Excl.t nat, Some ∅ : GsetK.t) : URA.prod _ _)).
+  Definition Ticket_locked r o := OwnM (Ticket_locked_ra r o).
 
-  Definition tklock_locked_ra (r : nat) (o : nat) : TicketLockRA :=
-    (maps_to_res r ((Auth.white (((Some o) : Excl.t nat, Some ∅ : GsetK.t) : URA.prod _ _), ε) : URA.prod _ _)).
-  Definition tklock_locked r o := OwnM (tklock_locked_ra r o).
+  Definition Ticket_issued_ra (r : nat) (m tid k : nat) : TicketRA :=
+    maps_to_res r (Auth.white ((ε : Excl.t nat, Some {[m]} : GsetK.t) : URA.prod _ _)).
+  Definition Ticket_issued r m tid k := OwnM (Ticket_issued_ra r m tid k).
 
-  (* The issuing thread holds my ticket -> (my thread id, and my obligation id). *)
-  Definition tklock_issued_ra (r : nat) (m tid k : nat) : TicketLockRA :=
-    (maps_to_res r ((Auth.white ((ε : Excl.t nat, Some {[m]} : GsetK.t) : URA.prod _ _), AuExAnyW_ra m (tid, k)) : URA.prod _ _)).
-  Definition tklock_issued r m tid k := OwnM (tklock_issued_ra r m tid k).
-
-  (* The invariant holds ticket -> (thread id, obligation id) for the waiting threads. *)
-  Definition tklock_wait_ra (r : nat) (m tid k : nat) : TicketLockRA :=
-    (maps_to_res r ((Auth.white ((ε : Excl.t nat, Some ∅ : GsetK.t) : URA.prod _ _), AuExAnyB_ra m (tid, k)) : URA.prod _ _)).
-  Definition tklock_wait r m tid k := OwnM (tklock_wait_ra r m tid k).
-
-
+  Lemma Ticket_alloc o D :
+    TicketRA_Auth ⊢ |==> TicketRA_Auth ∗ (∃ r, Ticket_black r o D ∗ Ticket_locked r o).
+  Proof.
+    iIntros "[%U BASE]".
+    assert (URA.updatable
+      ((λ k, if lt_dec k U then ε else TicketRA_Auth_base) : TicketRA)
+      (((λ k, if lt_dec k (S U) then ε else TicketRA_Auth_base) : TicketRA)
+        ⋅ (maps_to_res U TicketRA_Auth_base))) as UPD.
+    { ur. apply pointwise_updatable. i. unfold maps_to_res. des_ifs; try lia.
+      - rewrite URA.unit_idl. reflexivity.
+      - rewrite URA.unit_idl. reflexivity.
+      - rewrite URA.unit_id. reflexivity.  }
+    iMod (OwnM_Upd with "BASE") as "[A B]". apply UPD.
+    assert (URA.updatable
+      (maps_to_res U TicketRA_Auth_base)
+      (Ticket_black_ra U o D
+        ⋅ maps_to_res U (Auth.white ((Some o : Excl.t nat, Some D : GsetK.t) : URA.prod _ _)))).
+    { ur. apply pointwise_updatable. i.
+      unfold Ticket_black_ra, Ticket_locked_ra, maps_to_res, TicketRA_Auth_base.
+      des_ifs; cycle 1. rewrite URA.unit_id. reflexivity.
+      apply Auth.auth_update. ii. des. split. ur. split; ur; auto.
+      ur in FRAME. des_ifs. ur in H1. des_ifs. ur in H0. des_ifs. ur. f_equal. ur. auto.
+      set_unfold. ur. des_ifs. f_equal. set_solver. set_solver. }
+    iMod (OwnM_Upd with "B") as "[C D]". apply H.
+    assert (URA.updatable
+      (maps_to_res U (Auth.white ((Some o : Excl.t nat, Some D : GsetK.t) : URA.prod _ _)))
+      (maps_to_res U (Auth.white ((Some o : Excl.t nat, Some ∅ : GsetK.t) : URA.prod _ _)))).
+    { apply maps_to_updatable. etrans.
+      { apply Auth.auth_dup_white. instantiate (1:=(ε, Some ∅)). ur. f_equal; ur; des_ifs.
+        f_equal. set_solver. set_solver. }
+      rewrite <- URA.unit_id. apply URA.updatable_add; cycle 1. apply URA.updatable_unit.
+      ii. ur in H0. des_ifs.
+      { destruct f0. ur in H0. des. ur in H0. des_ifs.
+        ur in H1. des_ifs. ur. rewrite unfold_prod_add. ur. split; ur; auto.
+        des_ifs. set_solver. }
+      { des. ur. split; auto. destruct H0. destruct x.
+        exists (c, c0 ⋅ Some D). repeat (rewrite unfold_prod_add; des_ifs). f_equal.
+        destruct c4; destruct c0; ur; des_ifs; ss; des_ifs. f_equal. all:set_solver. } }
+    iMod (OwnM_Upd with "D") as "E". apply H0.
+    iModIntro. iSplitL "A".
+    { iExists (S U). auto. }
+    { iExists U. iSplitL "C". auto. unfold Ticket_locked, Ticket_locked_ra. auto. }
+    
   (** Properties. *)
-
   (* TODO : prove lemmas. *)
+  Lemma ticketlockB_alloc :
+    TicketLockRA_Auth ⊢ |==> (TicketLockRA_Auth ∗ (∃ r, tklockB r 0 ∅ ∗ tklock_locked r 0)).
+  Proof.
+    iIntros "[%U BASE]". iModIntro. iSplitL.
+    { iExists (S U). }
 
-End TKLOCK.
+End Ticket.
+Section TICKETS.
+  Definition TicketsRA : URA.t := (nat ==> AuthExclAnysRA)%ra.
+  
+End TICKETS.
